coq-minuska/theories/builtin/empty.v
@@ -4,65 +4,16 @@ From Minuska Require Import
     ocaml_interface
 .
 
+Definition void_value_algebra (NV Sy : Type)
+    : ValueAlgebra void NV Sy void void
+:= {|
+    builtin_function_interp
+        := fun _ _ _ => None ;
+    builtin_predicate_interp
+        := fun _ _ _ => None ;
+|}    .
 
-Inductive Emptyset : Set := .
-
-#[export]
-Instance emptyset_eqdec : EqDecision Emptyset.
-Proof.
-    intros x y.
-    destruct x, y.
-Defined.
-
-#[export]
-Program Instance emptyset_fin : Finite Emptyset := {|
-    enum := [];
-|}.
-Next Obligation.
-    constructor.
-Qed.
-Next Obligation.
-    destruct x.
-Qed.
-Fail Next Obligation.
-
-
-Section sec.
-
-    Context
-        {TermSymbol : Set}
-        {TermSymbols : Symbols TermSymbol}
-    .
-
-    #[local]
-    Program Instance mysignature : Signature := {|
-        FunSymbol
-            := Emptyset ;
-        PredSymbol
-            := Emptyset ;
-    |}.
-    Fail Next Obligation.
-
-    Program Definition βover
-        : ModelOver mysignature MyUnit Emptyset := {|
-        builtin_function_interp
-            := fun _ _ _ => None ;
-        builtin_predicate_interp
-            := fun _ _ _ => None ;
-    |}.
-    Fail Next Obligation.
-
-    #[local]
-    Instance β
-        : @Model _ _ mysignature MyUnit := {|
-        BasicValue
-            := Emptyset ;
-        builtin_model_over := βover ;
-    |}.
-
-End sec.
-
-Definition bindings (Q : Type) : string -> SymbolInfo Emptyset void Emptyset void Q void
+Definition bindings (Q : Type) : string -> SymbolInfo void void void void Q void
 :=
     fun s => si_none _ _ _ _ _ _
 .
