coq-minuska/theories/builtin/example_list_int_model.v
@@ -10,15 +10,14 @@ From Minuska Require Import
 
 
 Example example_list_int_model_1
-    {TermSymbol : Type}
-    {TermSymbols : Symbols TermSymbol}
+    (TermSymbol : Type)
     (NondetValue : Type)
     :
-    Model list_signature NondetValue
+    ValueAlgebra (bool+(simple_list_carrier Z)) NondetValue TermSymbol ListFunSymbol ListPredSymbol
 :=
-    model_of_relaxed (
-        rmf_apply list_relaxed_functor (
-            int_relaxed_model TermSymbol TermSymbols NondetValue
-        )
+    small_model_of_relaxed (
+        list_wrapper _ _ _ _ _ _ (int_relaxed_va TermSymbol NondetValue)
     )
 .
+
+(* About example_list_int_model_1. *)
